\begin{itemize}
	\item [a) ] $\vec{u}+\vec{v} = \begin{bmatrix} 1+2 \\ 3+5 \end{bmatrix}$ = $\begin{bmatrix} 3\\ 8 \end{bmatrix}$
	\item [b) ] $\vec{u}-\vec{v} = \begin{bmatrix}1-2 \\ 3-5 \end{bmatrix}$ = $\begin{bmatrix}\text{-}1 \\ \text{-}2 \end{bmatrix}$
	\item [c) ] $3\vec{u}+\vec{v} = \begin{bmatrix} 3*1 + 2 \\ 3*3 + 5\end{bmatrix}$ = $\begin{bmatrix} 5 \\ 14\end{bmatrix}$
	\item [d) ] $2(\vec{v}-2\vec{u}) =\begin{bmatrix} 2*(2-2*1) \\ 2*(5-2*3)\end{bmatrix}$ =$\begin{bmatrix} 0 \\ \text{-}2\end{bmatrix}$
	\item [e) ] $4\vec{u}-2(\vec{u}-3\vec{v}) = \begin{bmatrix}4*1-2*(1-3*2) \\ 4*3-2*(3-3*5)\end{bmatrix} = \begin{bmatrix}14\\ 36\end{bmatrix}$
\end{itemize}
