\begin{enumerate}
\item $u+v = \begin{bmatrix} 1+2 \\ 3+5 \end{bmatrix}$ = $\begin{bmatrix} 3\\ 8 \end{bmatrix}$
\item $u-v = \begin{bmatrix}1-2 \\ 3-5 \end{bmatrix}$ = $\begin{bmatrix}\text{-}1 \\ \text{-}2 \end{bmatrix}$
\item $3u+v = \begin{bmatrix} 3*1 + 2 \\ 3*3 + 5\end{bmatrix}$ = $\begin{bmatrix} 5 \\ 14\end{bmatrix}$
\item $2(v-2u) =\begin{bmatrix} 2*(2-2*1) \\ 2*(5-2*3)\end{bmatrix}$ =$\begin{bmatrix} 0 \\ \text{-}2\end{bmatrix}$
\item $4u-2(u-3v) = \begin{bmatrix}4*1-2*(1-3*2) \\ 4*3-2*(3-3*5)\end{bmatrix} = \begin{bmatrix}14\\ 36\end{bmatrix}$
\end{enumerate}
