\begin{itemize}
\item[a) ] $\alpha = \arccos{\frac{||\vec{u}|| \cdot ||\vec{v}||}{\vec{u} \cdot \vec{v}}} = \arccos{\frac{6}{12}}=\arccos{0.5}=60^{\circ}$ 
\item[b) ] $\vec{v_{L}}=\frac{\vec{u}\cdot\vec{v}}{\vec{u}\cdot\vec{u}}\vec{u}=\frac{6}{18}\begin{bmatrix}3 \\ 3 \end{bmatrix}= \begin{bmatrix}1 \\ 1 \end{bmatrix}$
\item[c) ] $\vec{w_{L}}=\frac{\vec{u}\cdot\vec{w}}{\vec{u}\cdot\vec{u}}\vec{u}=\frac{-12}{18}\begin{bmatrix}3 \\ 3 \end{bmatrix}= \begin{bmatrix}-2 \\ -2 \end{bmatrix}$
\item[d) ] $||\vec{v_{L}}||= \sqrt{2},\ ||\vec{w_{L}}||=2\sqrt{2} $
\item[e) ] $\vec{v_{L}}=\frac{\vec{u}\cdot\vec{v}}{\vec{u}\cdot\vec{u}}\vec{u}\ :\ \{ \vec{v}=\begin{bmatrix}1 \\ 0 \end{bmatrix},\ \vec{u}=\begin{bmatrix}0 \\ 1 \end{bmatrix}\} =\frac{0}{1}\begin{bmatrix}0 \\ 1 \end{bmatrix}= \begin{bmatrix}0 \\ 0 \end{bmatrix}$
\item[f) ] $\vec{v_{S}}=2\vec{v_{L}}-\vec{v}\ :\ \{ \vec{v}=\begin{bmatrix}1 \\ 0 \end{bmatrix},\ \vec{u}=\begin{bmatrix}0 \\ 1 \end{bmatrix} \} = 2\begin{bmatrix}0 \\ 0 \end{bmatrix}- \begin{bmatrix}1 \\ 0 \end{bmatrix}= \begin{bmatrix}-1 \\ 0 \end{bmatrix}= \vec{-v}$
\end{itemize}